Tracing Support

src/Gen.v
@@ -29,6 +29,7 @@ Import ListNotations.
 Import RiscvMachine.
 
 From StackSafety Require Import MachineImpl.
+From StackSafety Require Import SubroutineSimple.
 
 From RecordUpdate Require Import RecordSet.
 Import RecordSetNotations.
@@ -140,25 +141,8 @@ Definition listify2 {A B} `{Show A} `{Show B}
 Instance ShowWord : Show word :=
   {| show x := show (word.signed x) |}.
 
-Definition printGPRs (m : MachineState) (p : PolicyState) :=
-  List.fold_right (fun '(rID, rVal, rTag) acc =>
-                     show rID ++ " : " ++ show rVal ++ " @ " ++ show rTag ++ nl ++ acc)%string ""
-                  (listify2 (getRegs m) (regtags p)). 
-
-Definition listify1_word mem := 
-  List.rev
-    (map.fold
-       (fun acc k v =>
-          (* Keep mod 4 *)
-          if Z.eqb (snd (Z.div_eucl (word.unsigned k) 4)) 0
-          then
-            let val := 
-                match loadWord mem k with
-                | Some w32 => LittleEndian.combine _ w32
-                | _ => 42424242
-                end in
-            (word.unsigned k,val) :: acc
-          else acc) nil mem).
+Definition printPC (m : MachineState) (p : PolicyState) :=
+  (show (word.unsigned (getPc m)) ++ " @ " ++ show (pctags p))%string.
 
 Definition CodeMap_Impl := Zkeyed_map CodeStatus.
 Definition CodeMap_fromImpl (cm : CodeMap_Impl) : CodeMap :=
@@ -176,46 +160,102 @@ Instance ShowCodeAnnotation : Show CodeAnnotation :=
        | normal => "normal"
        | _  => "ret"
        end |}.
-Derive Show for CodeStatus.
 
-Definition printMem (m : MachineState) (p : PolicyState) (cm : CodeMap_Impl) (i : LayoutInfo) :=
+Derive Show for CodeStatus.
+Derive Show for StackDomain.
+
+
+Definition printComponent (k : Component)
+           (m : MachineState) (p : PolicyState)
+           (cm : CodeMap_Impl) (c : context)
+           (i : LayoutInfo) :=
+  let val := proj m k in
+  let tag := pproj p k in
+  match k with
+  | Mem a =>
+    (* Check if in instruction memory *)
+    if andb (Z.leb (instLo i) a) (Z.leb a (instHi i))
+    then
+      match decode RV32I val with
+      | IInstruction inst =>
+        (show inst ++ " @ " ++ show tag ++ " < " ++ show (CodeMap_fromImpl cm a) ++ " > - " ++ show (fst c (Mem a)))%string
+      | _ => (show val ++ " <not-inst>")%string
+      end
+    else
+      (show val ++ " @" ++ show tag ++ " < " ++ show (CodeMap_fromImpl cm a) ++ " > - " ++ show (fst c (Mem a)))%string
+  | Reg r => 
+    ("r" ++ show r ++ " : " ++ show val ++ " @ " ++ show tag) %string
+  | PC => ("PC: " ++ printPC m p ++ " - " ++
+      match decode RV32I (proj m (Mem val)) with
+      | IInstruction inst =>
+        (show inst)
+      | _ => (show val ++ " <not-inst>")%string
+      end)%string
+  end.
+
+
+Definition printGPRs (m : MachineState) (p : PolicyState) :=
+  List.fold_left (fun acc '(rID, rVal, rTag) =>
+                     show rID ++ " : " ++ show rVal ++ " @ " ++ show rTag ++ nl ++ acc)%string 
+                  (listify2 (getRegs m) (regtags p)) "". 
+
+Definition listify1_word mem := 
+  List.rev
+    (map.fold
+       (fun acc k v =>
+          (* Keep mod 4 *)
+          if Z.eqb (snd (Z.div_eucl (word.unsigned k) 4)) 0
+          then
+            let val := 
+                match loadWord mem k with
+                | Some w32 => LittleEndian.combine _ w32
+                | _ => 42424242
+                end in
+            (word.unsigned k,val) :: acc
+          else acc) nil mem).
+
+Definition printMem (m : MachineState) (p : PolicyState) (cm : CodeMap_Impl) (c : context) (i : LayoutInfo) :=
   let mem := getMem m in
   let tags := memtags p in
   let mts := combine_match (listify1_word mem) (listify1 tags) in
-  List.fold_right
-    (fun '(k,val,t) s =>
+  List.fold_left
+    (fun s '(k,val,t) =>
        let printed :=
            if andb (Z.leb (instLo i) k)
                    (Z.leb k (instHi i))
            then
              match decode RV32I val with
              | IInstruction inst =>
-               (show inst ++ " @ " ++ show t ++ " < " ++ show (CodeMap_fromImpl cm k) ++ " >")%string
+               (show inst ++ " @ " ++ show t ++ " < " ++ show (CodeMap_fromImpl cm k) ++ " > - " ++ show (fst c (Mem k)))%string
              | _ => (show val ++ " <not-inst>")%string
              end
            else
-             (show val ++ " @" ++ show t ++ " < " ++ show (CodeMap_fromImpl cm k) ++ " >")%string in
+             (show val ++ " @" ++ show t ++ " < " ++ show (CodeMap_fromImpl cm k) ++ " > - " ++ show (fst c (Mem k)))%string in
        if andb (Z.eqb val 0) (seq.nilp t) then
          s
-       else
+       else 
        (show k ++ " : " ++ printed ++ nl ++ s)%string
-    ) "" mts.
-
-Definition printPC (m : MachineState) (p : PolicyState) :=
-  (show (word.unsigned (getPc m)) ++ " @ " ++ show (pctags p))%string.
+    ) mts "".
 
 Definition printMachine
-           (m : MachineState) (p : PolicyState) cm := (
+           (m : MachineState) (p : PolicyState) cm c := (
   "PC:" ++  
   printPC m p ++ nl ++
   "Registers:" ++ nl ++
   printGPRs m p ++ nl ++
   "Memory: " ++ nl ++
-  printMem m p cm defLayoutInfo ++ nl
+  printMem m p cm c defLayoutInfo ++ nl
   )%string.
 
+Definition defstackmap (i : LayoutInfo) (a : Addr) :=
+  if (andb (Z.leb (stackLo i) a)
+           (Z.leb a (stackHi i)))
+  then
+    true
+  else false.
+
 Instance ShowMP : Show (MachineState * PolicyState * CodeMap_Impl):=
-  {| show := fun '(m,p,cm) => printMachine m p cm |}.
+  {| show := fun '(m,p,cm) => "" (*printMachine m p cm (initC (defstackmap defLayoutInfo) m) *) |}.
 
 (*
 , initGPR :: TagSet 
@@ -434,6 +474,8 @@ Definition genInstr (i : LayoutInfo) (t : TagInfo)
  *)
 
 
+
+
 Definition headerHead offset f :
   list (InstructionI * TagSet * FunID * CodeAnnotation) := [(Jal ra offset , [Tinstr; Tcall], f    , call)].
 
@@ -442,6 +484,8 @@ Definition headerSeq offset f nextF :
   headerHead offset f ++
   [ (Sw sp ra 0    , [Tinstr; Th1]  , nextF, normal)
   ; (Addi sp sp 12 , [Tinstr; Th2]  , nextF, normal)
+  ; (Sw sp r0 (-8) , [Tinstr; Th3]  , nextF, normal)
+  ; (Sw sp r0 (-4) , [Tinstr; Th4]  , nextF, normal)        
   ].
 (* Based on Rob's 
   (* 08 *) IInstruction (Sw SP RA 0); (* H1 *)
@@ -485,7 +529,7 @@ genCall pplus ms ps dataP codeP callP genInstrTag headerSeq = do
                   match map.get cm (word.unsigned (getPc m) + i) with
                   | Some (inFun _ _) =>
                     (headerHead i f) 
-                  | _ => exception ("genCall - nofid: " ++ show (word.unsigned (getPc m) + i) ++ nl ++ printMachine m p cm)%string
+                  | _ => exception ("genCall - nofid: " ++ show (word.unsigned (getPc m) + i) ++ nl ++ printMachine m p cm (initC (defstackmap l) m))%string
                   end) existingSites  in
   let newOpts :=
       List.map (fun i => headerSeq i f nextF) newCallSites in
@@ -624,7 +668,7 @@ Fixpoint gen_exec_aux (steps : nat)
           end
         )
       | _ =>
-        trace ("Existing instruction mid-sequence" ++ nl)%string
+        (*trace ("Existing instruction mid-sequence" ++ nl)%string*)
               (ret (m0, p0, cm))
       end
    | _ =>
@@ -767,9 +811,7 @@ Definition genMach :=
   genMachine defLayoutInfo defTagInfo zeroedRiscvMachine zeroedPolicyState map.empty
              dataP codeP callP genInstrTag.
 
-From StackSafety Require Import SubroutineSimple.
-
-(* Sample1 (genMach). *)
+(* Sample1 (genMach).  *)
 
 (* Property with printing. *)
 
@@ -778,7 +820,7 @@ Derive Show for Component.
 Instance ShowValue : Show Value :=
   {| show v := show v |}.
 
-Fixpoint walk (ks : list Component) cm m p (c : context) m' (p' : PolicyState) (c' : context)
+Fixpoint walk (ks : list Component) cm m p (c : context) m' (p' : PolicyState) (c' : context) (traceOut : list (unit -> string))
          (cont : unit -> Checker) : Checker :=
   match ks with
   | [] => cont tt
@@ -786,41 +828,54 @@ Fixpoint walk (ks : list Component) cm m p (c : context) m' (p' : PolicyState) (
     match fst c k with
     | Sealed _ =>
       if Z.eqb (proj m k) (proj m' k)
-      then walk ks' cm m p c m' p' c' cont
-      else whenFail ("Integrity failure at component: " ++ show k ++ nl ++
+      then walk ks' cm m p c m' p' c' traceOut cont
+      else whenFail ("Initial Machine:" ++ nl ++
+                     concatStr (List.rev (List.map (fun f => f tt) traceOut)) ++
+                     "Integrity failure at component: " ++ show k ++ nl ++
                                                         "Component values: " ++ show (proj m k) ++ " vs " ++ show (proj m' k) ++ nl ++
-                                                        printMachine m p cm)%string false
-    | _ => walk ks' cm m p c m' p' c' cont
+                    "Final state: " ++ nl ++
+                    printMachine m p cm c)%string false
+    | _ => walk ks' cm m p c m' p' c' traceOut cont
     end
   end.
 
-Definition prop_SimpleStackIntegrityStep fuel m p cm ctx
+Derive Show for Observation.
+
+
+Definition calcTraceDiff cm (m m' : MachineState) (p p' : PolicyState) (c c' : context) (i : LayoutInfo) (o : Observation) : unit -> string :=
+  let compsToTrace :=
+      List.filter (fun k =>
+                 negb (andb (Z.eqb (proj m k) (proj m' k))
+                            (TagSet_eqb (pproj p k) (pproj p k)))) (getComponents m')  in
+  (fun tt => 
+    ("Observation: " ++ show o ++ nl ++
+    concatStr (List.map (fun k => printComponent k m' p' cm c' i ++ nl) compsToTrace) ++ nl)%string).
+                            
+
+Definition prop_SimpleStackIntegrityStep fuel i m p cm ctx
   : Checker.Checker :=
-  let fix aux fuel m p ctx : Checker.Checker :=
+  let fix aux fuel m p ctx traceOut : Checker.Checker :=
       match fuel with
       | O => collect "Out-of-Fuel" true
       | S fuel' => 
         match mpcstep (updateC (CodeMap_fromImpl cm)) (m,p,ctx) with
-        | None => collect "Failstop" true
+        | None => collect ("Failstop", fuel) true
         | Some (m', p', c', o) =>
+          let traceDiff :=
+              calcTraceDiff cm m m' p p' ctx c' i o in
           walk (getComponents m') cm m p ctx m' p' c'
-               (fun tt => aux fuel' m' p' c')
+               (traceDiff :: traceOut)
+               (fun tt => aux fuel' m' p' c' (traceDiff :: traceOut))
         end
       end in
-  aux fuel m p ctx.
-
-Definition defstackmap (i : LayoutInfo) (a : Addr) :=
-  if (andb (Z.leb (stackLo i) a)
-           (Z.leb a (stackHi i)))
-  then
-    true
-  else false.
+  aux fuel m p ctx ([fun tt => printMachine m p cm ctx]).
 
 Definition prop_integrity :=
   let sm := defstackmap defLayoutInfo in
   forAll genMach (fun '(m,p,cm) =>
-                    (prop_SimpleStackIntegrityStep 42 m p cm (initC sm m))).
+                    (prop_SimpleStackIntegrityStep 42 defLayoutInfo m p cm (initC sm m))).
 
 Extract Constant defNumTests => "1000".
 QuickCheck prop_integrity. 
+
 
